coq/proof/SoundForget.v
@@ -28,78 +28,6 @@ Require Import Inject. (* TODO: for simtac *)
 
 Set Implicit Arguments.
 
-(* ForgetUnique *)
-
-Lemma forget_unique_sound
-      conf_src st0_src d_src l_src
-      conf_tgt st0_tgt d_tgt l_tgt
-      invst invmem inv0
-      (STATE: InvState.Rel.sem conf_src conf_tgt st0_src st0_tgt invst invmem inv0)
-  : <<STATE_FORGET_UNIQUE: InvState.Rel.sem conf_src conf_tgt st0_src st0_tgt
-                                            invst invmem (ForgetUnique.t d_src d_tgt l_src l_tgt inv0)>>.
-Proof.
-  red. unfold ForgetUnique.t.
-  inv STATE.
-  econs; eauto; [inv SRC | inv TGT];
-    econs; eauto;
-    intros x IN; apply UNIQUE; ss;
-    apply AtomSetFacts.filter_iff in IN; try by solve_compat_bool;
-    des; eauto.
-Qed.
-
-Definition unary_no_leaks defs leaks inv0: Prop :=
-  forall x,
-    AtomSetImpl.mem x (AtomSetImpl.union defs leaks) = true ->
-    AtomSetImpl.mem x inv0.(Invariant.unique) = false.
-
-Lemma forget_unique_unary_no_leaks defs leaks inv0:
-  unary_no_leaks defs leaks (ForgetUnique.unary defs leaks inv0).
-Proof.
-  unfold unary_no_leaks. ii.
-  ss. rewrite AtomSetFacts.filter_b; try by solve_compat_bool.
-  apply andb_false_iff. right.
-  apply negb_false_iff. eauto.
-Qed.
-
-Lemma unary_no_leaks_Subset
-      defs leaks inv0 inv1
-      (SUBSET: Invariant.Subset_unary inv1 inv0)
-      (NO_LEAKS: unary_no_leaks defs leaks inv0)
-  : unary_no_leaks defs leaks inv1.
-Proof.
-  unfold unary_no_leaks in *.
-  i. exploit NO_LEAKS; eauto. i.
-  inv SUBSET. eauto.
-  destruct (AtomSetImpl.mem x (Invariant.unique inv1)) eqn:MEM; ss.
-  apply AtomSetFacts.mem_iff in MEM.
-  apply SUBSET_UNIQUE in MEM.
-  apply AtomSetFacts.mem_iff in MEM.
-  congruence.
-Qed.
-
-(* TODO: if not needed, delete *)
-
-Lemma forget_unique_unary_Subset
-      defs leaks inv0
-  : Invariant.Subset_unary (ForgetUnique.unary defs leaks inv0) inv0.
-Proof.
-  unfold ForgetUnique.unary.
-  econs; ss; ii.
-  - split; ss.
-  - eapply AtomSetFacts.filter_iff in H; try by solve_compat_bool.
-    des. eauto.
-Qed.
-
-Lemma forget_unique_Subset
-      def_src leaks_src
-      def_tgt leaks_tgt
-      inv0
-  : Invariant.Subset (ForgetUnique.t def_src def_tgt leaks_src leaks_tgt inv0) inv0.
-Proof.
-  unfold ForgetUnique.t.
-  econs; ss;
-    try apply forget_unique_unary_Subset.
-Qed.
 
 (* Forget *)
 
@@ -209,8 +137,8 @@ Proof.
 Qed.
 
 Lemma forget_unary_Subset
-      defs inv0
-  : Invariant.Subset_unary (Forget.unary defs inv0) inv0.
+      defs leaks inv0
+  : Invariant.Subset_unary (Forget.unary defs leaks inv0) inv0.
 Proof.
   unfold Forget.unary.
   econs; ss; ii.
@@ -221,13 +149,16 @@ Proof.
       des. eauto.
     + eapply PtrPairSetFacts.filter_iff in H; try by solve_compat_bool.
       des. eauto.
+  - eapply AtomSetFacts.filter_iff in H; try by solve_compat_bool.
+    des. eauto.
   - eapply IdTSetFacts.filter_iff in H; try by solve_compat_bool.
     des. eauto.
 Qed.
 
 Lemma forget_Subset
       def_src def_tgt inv0
-  : Invariant.Subset (Forget.t def_src def_tgt inv0) inv0.
+      leaks_src leaks_tgt
+  : Invariant.Subset (Forget.t def_src def_tgt leaks_src leaks_tgt inv0) inv0.
 Proof.
   unfold Forget.t.
   econs; ss;
@@ -238,18 +169,19 @@ Qed.
 
 (* soundness *)
 
-Definition unique_holds conf st inv: Prop :=
-  forall u, AtomSetImpl.mem u inv.(Invariant.unique) ->
-            InvState.Unary.sem_unique conf st u.
+Definition unique_preserved_except conf inv st1 except_for : Prop :=
+  forall u (MEM: AtomSetImpl.mem u inv.(Invariant.unique) = true)
+         (NO_LEAK: AtomSetImpl.mem u except_for = false),
+    InvState.Unary.sem_unique conf st1 u.
 
 Lemma forget_unary_sound
-      conf defs st0 st1
+      conf defs leaks st0 st1
       inv invst invmem
       (EQUIV : state_equiv_except defs st0 st1)
-      (UNIQUE : unique_holds conf st1 inv)
+      (UNIQUE : unique_preserved_except conf inv st1 (AtomSetImpl.union defs leaks))
       (STATE : InvState.Unary.sem conf st0 invst invmem inv)
       (WF_LC: memory_props.MemProps.wf_lc st1.(Mem) st1.(EC).(Locals))
-  : InvState.Unary.sem conf st1 invst invmem (Forget.unary defs inv).
+  : InvState.Unary.sem conf st1 invst invmem (Forget.unary defs leaks inv).
 Proof.
   inv STATE.
   assert (EQUIV_REV: state_equiv_except defs st1 st0).
@@ -278,7 +210,14 @@ Proof.
       solve_negb_liftpred.
       exploit sem_valueT_equiv_except; try exact EQUIV_REV; try exact VAL1; eauto. i. des.
       exploit sem_valueT_equiv_except; try exact EQUIV_REV; try exact VAL2; eauto.
-  - ii. ss. apply UNIQUE. apply AtomSetFacts.mem_iff. eauto.
+  - ii. ss.
+    apply AtomSetFacts.filter_iff in H; [| solve_compat_bool]. des.
+    apply negb_true_iff in H0.
+
+    unfold unique_preserved_except in *.
+
+    apply UNIQUE; eauto.
+    apply AtomSetFacts.mem_iff; eauto.
   - ii. ss.
     apply IdTSetFacts.filter_iff in H; [| solve_compat_bool]. des.
     unfold flip, compose in *.
@@ -297,15 +236,16 @@ Lemma forget_sound
       st1_src st1_tgt
       invst invmem inv0
       defs_src defs_tgt
+      leaks_src leaks_tgt
       (STATE: InvState.Rel.sem conf_src conf_tgt st0_src st0_tgt invst invmem inv0)
       (EQUIV_SRC: state_equiv_except defs_src st0_src st1_src)
       (EQUIV_TGT: state_equiv_except defs_tgt st0_tgt st1_tgt)
-      (UNIQUE_SRC: unique_holds conf_src st1_src inv0.(Invariant.src))
-      (UNIQUE_TGT: unique_holds conf_tgt st1_tgt inv0.(Invariant.tgt))
+      (UNIQUE_SRC: unique_preserved_except conf_src inv0.(Invariant.src) st1_src (AtomSetImpl.union defs_src leaks_src))
+      (UNIQUE_TGT: unique_preserved_except conf_tgt inv0.(Invariant.tgt) st1_tgt (AtomSetImpl.union defs_tgt leaks_tgt))
       (WF_LC_SRC: memory_props.MemProps.wf_lc st1_src.(Mem) st1_src.(EC).(Locals))
       (WF_LC_TGT: memory_props.MemProps.wf_lc st1_tgt.(Mem) st1_tgt.(EC).(Locals))
   : <<STATE_FORGET: InvState.Rel.sem conf_src conf_tgt st1_src st1_tgt
-                            invst invmem (Forget.t defs_src defs_tgt inv0)>>.
+                            invst invmem (Forget.t defs_src defs_tgt leaks_src leaks_tgt inv0)>>.
 Proof.
   inv STATE.
   econs; ss.
@@ -325,3 +265,82 @@ Proof.
     + ii. exploit MAYDIFF; eauto.
     + ii. exploit MAYDIFF; eauto.
 Qed.
+
+(* unused *)
+
+(* (* ForgetUnique *) *)
+
+(* Lemma forget_unique_sound *)
+(*       conf_src st0_src d_src l_src *)
+(*       conf_tgt st0_tgt d_tgt l_tgt *)
+(*       invst invmem inv0 *)
+(*       (STATE: InvState.Rel.sem conf_src conf_tgt st0_src st0_tgt invst invmem inv0) *)
+(*   : <<STATE_FORGET_UNIQUE: InvState.Rel.sem conf_src conf_tgt st0_src st0_tgt *)
+(*                                             invst invmem (ForgetUnique.t d_src d_tgt l_src l_tgt inv0)>>. *)
+(* Proof. *)
+(*   red. unfold ForgetUnique.t. *)
+(*   inv STATE. *)
+(*   econs; eauto; [inv SRC | inv TGT]; *)
+(*     econs; eauto; *)
+(*     intros x IN; apply UNIQUE; ss; *)
+(*     apply AtomSetFacts.filter_iff in IN; try by solve_compat_bool; *)
+(*     des; eauto. *)
+(* Qed. *)
+
+(* Definition unary_no_leaks defs leaks inv0: Prop := *)
+(*   forall x, *)
+(*     AtomSetImpl.mem x (AtomSetImpl.union defs leaks) = true -> *)
+(*     AtomSetImpl.mem x inv0.(Invariant.unique) = false. *)
+(* (* TODO: forall x (LEAKS: mem ...) (UNIQUE: mem ...), False. *) *)
+
+(* Lemma forget_unique_unary_no_leaks defs leaks inv0: *)
+(*   unary_no_leaks defs leaks (ForgetUnique.unary defs leaks inv0). *)
+(*   (* TODO: unary_no_leaks (AtomSetImpl.union defs leaks) (ForgetUnique.unary defs leaks inv0). *) *)
+(* Proof. *)
+(*   unfold unary_no_leaks. ii. *)
+(*   ss. rewrite AtomSetFacts.filter_b; try by solve_compat_bool. *)
+(*   apply andb_false_iff. right. *)
+(*   apply negb_false_iff. eauto. *)
+(* Qed. *)
+
+(* Lemma unary_no_leaks_Subset *)
+(* (* TODO: Lemma unary_no_leaks_mon *) *)
+(*       defs leaks inv0 inv1 *)
+(*       (SUBSET: Invariant.Subset_unary inv1 inv0) *)
+(*       (NO_LEAKS: unary_no_leaks defs leaks inv0) *)
+(*   : unary_no_leaks defs leaks inv1. *)
+(* Proof. *)
+(*   unfold unary_no_leaks in *. *)
+(*   i. exploit NO_LEAKS; eauto. i. *)
+(*   inv SUBSET. eauto. *)
+(*   destruct (AtomSetImpl.mem x (Invariant.unique inv1)) eqn:MEM; ss. *)
+(*   apply AtomSetFacts.mem_iff in MEM. *)
+(*   apply SUBSET_UNIQUE in MEM. *)
+(*   apply AtomSetFacts.mem_iff in MEM. *)
+(*   congruence. *)
+(* Qed. *)
+
+(* (* TODO: if not needed, delete *) *)
+
+(* Lemma forget_unique_unary_Subset *)
+(*       defs leaks inv0 *)
+(*   : Invariant.Subset_unary (ForgetUnique.unary defs leaks inv0) inv0. *)
+(* Proof. *)
+(*   unfold ForgetUnique.unary. *)
+(*   econs; ss; ii. *)
+(*   - split; ss. *)
+(*   - eapply AtomSetFacts.filter_iff in H; try by solve_compat_bool. *)
+(*     des. eauto. *)
+(* Qed. *)
+
+(* Lemma forget_unique_Subset *)
+(*       def_src leaks_src *)
+(*       def_tgt leaks_tgt *)
+(*       inv0 *)
+(*   : Invariant.Subset (ForgetUnique.t def_src def_tgt leaks_src leaks_tgt inv0) inv0. *)
+(* Proof. *)
+(*   unfold ForgetUnique.t. *)
+(*   econs; ss; *)
+(*     try apply forget_unique_unary_Subset. *)
+(* Qed. *)
+
